\begin{MapleInput}
> restart; X:=[1,2,3,4]: Y:=[0,5,15,24]: f1:=x->a0+a1*x:
  S:=0: 
  for i from 1 to 4 do 
    S:=S+(f1(X[i])-Y[i])^2; 
  end do:
> fS:=unapply(S,(a0,a1));
\end{MapleInput}
\begin{MapleOutput}
{\it fS}\, := \,( {{\it a0},{\it a1}} )\mapsto  \left( {\it a0}+{\it a1} \right) ^{2}+ \left( {\it a0}+2\,{\it a1}-5 \right) ^{2}+ \left( {\it a0}+3\,{\it a1}-15 \right) ^{2}+ \left( {\it a0}+4\,{\it a1}-24 \right) ^{2}
\end{MapleOutput}
\begin{MapleInput}
> expand(fS(a0,a1));
\end{MapleInput}
\begin{MapleOutput}
4\,{{\it a0}}^{2}+20\,{\it a0}\,{\it a1}+30\,{{\it a1}}^{2}-88\,{\it a0}-302\,{\it a1}+826
\end{MapleOutput}

\begin{MapleInput}
> plot3d(fS(a0,a1),a0=-20..20,a1=0..20);
\end{MapleInput}
\MaplePlot{50mm}{./figures/C8_LeastSquareFitplot3d3.eps}


\begin{MapleInput}
> eqs:={diff(expand(S),a0)=0, diff(expand(S),a1)=0};
\end{MapleInput}
\begin{MapleOutput}
{\it eqs}\, := \, \left\{ 8\,{\it a0}+20\,{\it a1}-88=0,20\,{\it a0}+60\,{\it a1}-302=0 \right\}
\end{MapleOutput}

\begin{MapleInput}
> solve(eqs,{a0,a1});
\end{MapleInput}
\begin{MapleOutput}
\left\{ {\it a0}=-\frac{19}{2},{\it a1}={\frac {41}{5}} \right\}
\end{MapleOutput}
